src/cddl/test/dpe/CDDLTest.DPE.SignInput.fst
@@ -14,72 +14,77 @@ open CDDL.Pulse.AST.Bundle
 open CBOR.Spec.API.Type
 open CDDLTest.DPE.Common
 open CDDL.Spec.Base
+module DC = CDDLTest.DPE.DeriveContextInput
+open  CDDLTest.DPE.DeriveContextInput
 
-fn parse_option_bytes x (w:erased _) res
-requires
-  rel_option
-    rel_evercddl_bytes x w **
-  Trade.trade (rel_option rel_evercddl_bytes x w) res
-returns x:option (slice UInt8.t)
-ensures is_slice_opt x res
-{
-  rel_option_cases _ _ _;
-
-  match x {
-    None -> {
-      Trade.elim_trade _ _;
-      fold (is_slice_opt None res);
-      None
-    }
-
-    Some _ -> {
-      let sl = destruct_rel_option _ _ _;
-      Trade.trade_compose _ _ res;
-      let sl = extract_bytes _ _;
-      Trade.trade_compose _ _ res;
-      fold (is_slice_opt (Some sl) res);
-      Some sl
-    }
-  }
-}
-
-fn parse_sign_input x (w:erased _) res
-requires
-  rel_evercddl_signinputargs x w **
-  Trade.trade (rel_evercddl_signinputargs x w) res
-returns x:option (slice UInt8.t)
-ensures is_slice_opt x res
-{
-  unfold_with_trade (`%rel_evercddl_signinputargs) (rel_evercddl_signinputargs x w);
-  Trade.trade_compose _ _ res;
+ghost
+fn extract_to_be_signed x w
+requires rel_evercddl_signinputargs x w
+ensures 
+  rel_evercddl_bytes x.intkey5 w._x4 **
+  Trade.trade (rel_evercddl_bytes x.intkey5 w._x4)
+              (rel_evercddl_signinputargs x w)
+{ 
+  unfold_with_trade
+    (`%rel_evercddl_signinputargs) 
+    (rel_evercddl_signinputargs x w);
   destruct_rel_fun _ _ _ _ _;
-  Trade.trade_compose _ _ res;
-
-  let rest_5 = fst_pair_concrete _ _ _ _ _;
-  let tbs = snd_pair_concrete _ _ _ _ _;
-
-  rewrite each (Tactics.PrettifyType.named "intkey5" evercddl_bytes_pretty)
-      as evercddl_bytes_pretty;
-  parse_option_bytes _ _ res;
+  Trade.trade_compose _ _ (rel_evercddl_signinputargs x w);
+  fold_last_relation (`%tstr_any) tstr_any;  
+  let rest_5 = fst_pair _ _ _ _ _;
+  let tbs = snd_pair _ _ _ _ _;
+  with xx yy. assert (rel_evercddl_bytes xx yy);
+  rewrite each xx as x.intkey5, yy as w._x4;
+  ()
 }
+
+fn extract_to_be_signed_bytes x (w:erased _)
+requires rel_evercddl_signinputargs x w
+returns tbs:Slice.slice UInt8.t
+ensures exists* p s.
+  pts_to tbs #p s **
+  Trade.trade (pts_to tbs #p s)
+              (rel_evercddl_signinputargs x w) **
+  pure (bytes_of_evercddl_bytes s w._x4)
+{
+  extract_to_be_signed x w;
+  let tbs = extract_bytes _ _;
+  Trade.trade_compose _ _ (rel_evercddl_signinputargs x w);
+  tbs
+}
+
+let is_tbs_bytes (tbs_bytes:Seq.seq UInt8.t) (w:Seq.seq UInt8.t) =
+  exists (wx:spect_evercddl_signinputargs_pretty) (wr:Seq.seq UInt8.t).
+          validate_and_parse_postcond_some bundle_signinputargs.b_spec.parser w wx wr /\
+          wx._x4 == spect_evercddl_bytes_pretty_right (spect_evercddl_bstr_pretty_right tbs_bytes)
+
 
 fn parse_sign_input_args (s:Slice.slice UInt8.t) (#p:perm) (#w:erased _)
 requires pts_to s #p w
-returns x:option (slice UInt8.t)
-ensures is_slice_opt x (pts_to s #p w)
+returns tbs:option (Slice.slice UInt8.t)
+ensures (
+  match tbs with
+  | None -> pts_to s #p w
+  | Some tbs -> 
+    exists* #q tbs_bytes.
+      pts_to tbs #q tbs_bytes **
+      Trade.trade (pts_to tbs #q tbs_bytes) (pts_to s #p w) **
+      pure (is_tbs_bytes tbs_bytes w)
+)
 {
   let res = validate_and_parse_signinputargs s;
   match res {
     None -> {
       unfold validate_and_parse_post;
-      fold (is_slice_opt None (pts_to s #p w));
       None
     }
     Some xrem -> {
       let (x, rem) = xrem;
-      elim_validate_and_parse_post_some x rem;
+      unfold validate_and_parse_post;
       Trade.Util.elim_hyp_r _ _ _;
-      parse_sign_input _ _ _;
+      let tbs = extract_to_be_signed_bytes _ _;
+      Trade.trade_compose _ _ (pts_to s #p w);
+      Some tbs
     }
   }
 }
