src/cddl/test/dpe/CDDLTest.DPE.SignOutput.fst
@@ -1,0 +1,242 @@
+module CDDLTest.DPE.SignOutput
+module EqTest = CDDL.Spec.EqTest
+open CDDLTest.Test
+open Pulse.Lib
+open Pulse.Lib.Pervasives
+open CDDLTest.Destructors
+#lang-pulse
+open CDDL.Pulse.Parse.Base
+module S = Pulse.Lib.Slice
+module U8 = FStar.UInt8
+open CDDL.Pulse.Types
+module T = CDDL.Pulse.AST.Tactics
+open CDDL.Pulse.AST.Bundle
+open CBOR.Spec.API.Type
+open CDDL.Spec.Base
+open CDDLTest.DPE.Common
+
+let pretty_bytes (x:Seq.seq UInt8.t) =
+  spect_evercddl_bytes_pretty_right (spect_evercddl_bstr_pretty_right x)
+
+let pretty_slice (x:slice UInt8.t) =
+  evercddl_bytes_pretty_right (evercddl_bstr_pretty_right x)
+
+let _ = rel_evercddl_signoutputargs
+
+
+let struct_has_sig
+    (hres:spect_evercddl_signoutputargs_pretty) 
+    (sig :Seq.seq UInt8.t) =
+  hres._x0 == Some (pretty_bytes sig) /\
+  hres._x1 == None
+
+let of_bytes (#p:perm) (x:evercddl_bytes_pretty) (s:Slice.slice UInt8.t) =
+  let x = evercddl_bstr_pretty_left (evercddl_bytes_pretty_left x) in
+  x.s == s /\
+  x.p == p
+
+let of_bytes_option #p (x:option evercddl_bytes_pretty) (s:option (Slice.slice UInt8.t)) =
+  match x, s with
+  | None, None -> True
+  | Some x, Some s -> of_bytes #p x s
+  | _ -> False
+
+fn mk_evercddl_bytes_pretty
+    (x:Slice.slice UInt8.t)
+    (#p #w:erased _)
+requires
+  pts_to x #p w
+returns res:_
+ensures
+  rel_option rel_evercddl_bytes res (Some <| pretty_bytes w) **
+  pure (of_bytes_option #p res (Some x))
+{
+  let res : slice UInt8.t = { s = x; p = p };
+  rewrite (pts_to x #p w ** pure (false == false))
+  as (rel_option rel_evercddl_bytes (Some <| pretty_slice res) (Some <| pretty_bytes w));
+  Some (pretty_slice res)
+}
+
+fn mk_evercddl_bytes_pretty_none ()
+requires emp
+ensures
+  rel_option rel_evercddl_bytes None None
+{
+  rewrite emp as rel_option rel_evercddl_bytes None None;
+}
+
+[@@pulse_unfold]
+unfold
+let my_unfold_l (#a:Type) (s:list string) (p:a) = norm [delta_only s; iota; primops] p
+
+ghost
+fn fold_l (s:list string) (p:slprop)
+requires my_unfold_l s p
+ensures p
+{
+  norm_spec [delta_only s; iota; primops] p;
+  rewrite each (my_unfold_l s p) as p;
+}
+
+ghost
+fn unfold_l (s:list string) (p:slprop)
+requires p
+ensures my_unfold_l s p
+{
+  norm_spec [delta_only s; iota; primops] p;
+  rewrite each p as (my_unfold_l s p);
+}
+
+ghost
+fn mk_rel_pair (#a0 #b0 #a1 #b1:Type0) (r0:rel a0 b0) (r1:rel a1 b1) (x0:a0) (#y0:b0) (x1:a1) (#y1:b1)
+requires
+  r0 x0 y0 ** r1 x1 y1
+ensures
+  rel_pair r0 r1 (x0, x1) (y0, y1)
+{
+  rewrite (r0 x0 y0 ** r1 x1 y1)
+  as (rel_pair r0 r1 (x0, x1) (y0, y1));
+}
+
+ghost
+fn fold_rel_option (#a #b:Type0) (r:rel a b) (x:a) (y:b)
+requires
+  r x y
+ensures
+  rel_option r (Some x) (Some y)
+{
+  rewrite (r x y) as (rel_option r (Some x) (Some y));
+}
+
+ghost
+fn fold_sign_output_args (x:_) (w:erased _)
+requires
+  rel_pair (rel_option rel_evercddl_bytes) (rel_option rel_evercddl_bytes)
+          x w
+ensures 
+  rel_evercddl_signoutputargs
+    (evercddl_signoutputargs_pretty_right x)
+    (spect_evercddl_signoutputargs_pretty_right w)
+{
+  rewrite (rel_pair (rel_option rel_evercddl_bytes) (rel_option rel_evercddl_bytes)
+                  x w)
+  as (rel_evercddl_signoutputargs 
+             (evercddl_signoutputargs_pretty_right x)
+             (spect_evercddl_signoutputargs_pretty_right w));
+}
+
+let res_has_sig
+    (res:evercddl_signoutputargs_pretty)
+    (sig:Slice.slice UInt8.t) p =
+  of_bytes_option #p res.intkey1 (Some sig) /\
+  of_bytes_option #1.0R res.intkey2 None
+
+fn prepare_sign_output
+    (sign:Slice.slice UInt8.t)
+    (#s:erased _) (#p:perm)
+requires
+    pts_to sign #p s
+returns res:_
+ensures
+  exists* hres. 
+    rel_evercddl_signoutputargs res hres **
+    pure (struct_has_sig hres s /\
+          res_has_sig res sign p)
+{
+  let pk = mk_evercddl_bytes_pretty sign;
+  mk_evercddl_bytes_pretty_none ();
+  mk_rel_pair (rel_option rel_evercddl_bytes)
+              (rel_option rel_evercddl_bytes) _ None;
+  fold_sign_output_args _ _;
+  with res hres. assert (rel_evercddl_signoutputargs res hres);
+  res
+}
+ 
+let is_serialized_sign_output hres w =
+  exists sz.
+    impl_serialize_post (coerce_spec bundle_signoutputargs
+                .b_spec
+              spect_evercddl_signoutputargs_pretty
+              ())
+          hres
+          w
+          sz
+
+let norm_token = emp
+ghost
+fn intro_norm ()
+requires emp
+ensures norm_token
+{
+  fold norm_token;
+}
+
+ghost
+fn force_norm ()
+requires norm_token
+ensures emp
+{
+  unfold norm_token;
+}
+
+ghost 
+fn extract_bytes x (y:erased _)
+requires rel_evercddl_bytes x y
+returns xx:Slice.slice UInt8.t
+ensures 
+  exists* p yy. 
+    pts_to xx #p yy **
+    pure (bytes_of_evercddl_bytes yy y /\ of_bytes #p x xx)
+
+{
+  unfold_l [`%rel_fun; `%rel_evercddl_bytes; `%rel_evercddl_bstr; `%mk_rel; `%rel_slice_of_seq]
+            (rel_evercddl_bytes x y);
+  with (x:Slice.slice UInt8.t) #p y. assert S.pts_to x #p y;
+  x
+}
+
+ghost
+fn destruct_signoutputargs x hres sign p s
+requires
+    rel_evercddl_signoutputargs x hres **
+    pure (of_bytes_option #p x.intkey1 (Some sign) /\
+          of_bytes_option #1.0R x.intkey2 None /\
+          struct_has_sig hres s)
+ensures
+    pts_to sign #p s
+{
+  rewrite (rel_evercddl_signoutputargs x hres) as
+          (rel_evercddl_bytes (Some?.v x.intkey1) (Some?.v hres._x0) **
+           emp);
+  let xx = extract_bytes (Some?.v x.intkey1) _;
+  rewrite each xx as sign;
+  ()
+}
+
+fn write_certify_key_output_alt
+    (out:Slice.slice UInt8.t)
+    (sign:Slice.slice UInt8.t)
+    (#s:erased _) (#p:perm)
+requires
+  exists* w.
+    pts_to sign #p s **
+    pts_to out w
+returns res:bool
+ensures
+  exists* w.
+    pts_to sign #p s **
+    pts_to out w **
+    pure (exists hres. res ==> 
+          is_serialized_sign_output hres w /\
+          struct_has_sig hres s)
+{
+  let res = prepare_sign_output sign;
+  let sz = serialize_signoutputargs' _ out;
+  destruct_signoutputargs res _ sign p s;
+  if (sz = 0sz) {
+     false
+  }
+  else {
+    true
+  }
+}
